Implement Phoasify and Dephoasify at the level of Phoas_expr and prove their soundness

PyLevelLang/src/PyLevelLang/Phoas_Interpret.v
@@ -73,105 +73,105 @@ Section WithMap.
                                (fun v acc => phoasify (set_phoas_local (set_phoas_local env x v) y acc) fn)
       | ELet x e1 e2 => PhELet x (phoasify env e1) (fun v => phoasify (set_phoas_local env x v) e2)
       end.
-
-    (* Remove one occurrence of x from l if there is one.
-     * Auxiliary function for the definition of fresh' below *)
-    Fixpoint remove_one (x : string) (l : list string) : list string :=
-      match l with
-      | nil => nil
-      | h :: t => if eqb h x then t else h :: remove_one x t
-      end.
-
-    Lemma in_remove_one_len : forall (x : string) (l : list string),
-        In x l -> List.length l = S (List.length (remove_one x l)).
-    Proof.
-      intros. induction l.
-      - apply in_nil in H. exfalso. apply H.
-      - simpl in H. destruct (eqb a x) eqn:E.
-        + simpl. rewrite E. reflexivity.
-        + destruct H as [HL | HR].
-          * rewrite <- eqb_eq in HL. rewrite HL in E. discriminate.
-          * simpl. rewrite E. simpl. rewrite (IHl HR). reflexivity.
-    Qed.
-
-    Lemma in_remove_one : forall (x : string) (l : list string),
-        In x l -> forall (y : string), x = y \/ In x (remove_one y l).
-    Proof.
-      intros x l H. induction l.
-      - intros. apply in_nil in H. exfalso. exact H.
-      - intros y. simpl in H. destruct H as [HL | HR].
-        + destruct (eqb a y) eqn:E.
-          * rewrite eqb_eq in E. rewrite HL in E. left. exact E.
-          * right. simpl. rewrite E. simpl. left. exact HL.
-        + destruct (IHl HR) with (y := y) as [HL' | HR'].
-          * left. exact HL'.
-          * right. simpl. destruct (eqb a y) eqn:E.
-            { exact HR. }
-            { simpl. right. exact HR'. }
-    Qed.
-
-    (* Append "'"s to x until the resulting name is not in used.
-     * The initial call should have (budget = length used) *)
-    Fixpoint fresh' (budget : nat) (used : list string) (x : string) : string :=
-      (* We need budget as a decreasing argument for the function *)
-      match budget with
-      | O => x
-      | S n => match in_dec string_dec x used with
-               | left _ => fresh' n (remove_one x used) (x ++ "'")
-               | right _ => x
-               end
-      end.
-
-    (* Given a list of used names and a hint, return a fresh name *)
-    Definition fresh (used : list string) (x : string) : string :=
-      fresh' (List.length used) used x.
-
-    Lemma len_app : forall y, length y < length (y ++ "'").
-    Proof.
-      induction y; auto. simpl. apply Arith_prebase.lt_n_S_stt. apply IHy.
-    Qed.
-
-    Lemma fresh'_len : forall (budget : nat) (used : list string) (x : string),
-        length x <= length (fresh' budget used x).
-    Proof.
-      induction budget; intros.
-      - destruct used; unfold fresh'; constructor.
-      - destruct (in_dec string_dec x used) eqn:E.
-        + unfold fresh'. rewrite E.
-          apply Nat.le_trans with (m := length (x ++ "'")).
-          * pose proof (len_app x) as len_app_x.
-            apply Nat.lt_le_incl. exact len_app_x.
-          * apply (IHbudget (remove_one x used) (x ++ "'")%string).
-        + unfold fresh'; rewrite E; constructor.
-    Qed.
-
-    Lemma fresh'_is_fresh : forall (budget : nat) (used : list string) (x : string),
-        budget = List.length used -> ~ In (fresh' budget used x) used.
-    Proof.
-      induction budget; intros.
-      - destruct used.
-        + auto.
-        + discriminate.
-      - rewrite H. destruct (in_dec string_dec x used) as [ HL | HR ] eqn:E.
-        + assert (Hrm_len: S budget = S (List.length (remove_one x used))).
-          { rewrite H. apply in_remove_one_len. apply HL. }
-          injection Hrm_len as Hrm_len.
-          apply (IHbudget (remove_one x used)) with (x := (x ++ "'")%string) in Hrm_len as Hrm.
-          unfold not. intros. apply in_remove_one with (y := x) in H0 as [HL'|HR'].
-          * assert (HA : length (x ++ "'") <= length (fresh' (Datatypes.length used) used x)).
-            { unfold fresh'. rewrite <- H. rewrite E. apply fresh'_len. }
-            rewrite HL' in HA. apply Arith_prebase.le_not_lt_stt in HA.
-            apply HA. apply len_app.
-          * unfold fresh' in HR'. rewrite <- H in HR'. rewrite E in HR'.
-            apply Hrm. unfold fresh'. apply HR'.
-        + unfold fresh'. rewrite <- H. rewrite E. exact HR.
-    Qed.
-
-    Corollary fresh_is_fresh : forall (used : list string) (x : string), ~ In (fresh used x) used.
-    Proof.
-      intros. unfold fresh. apply fresh'_is_fresh. reflexivity.
-    Qed.
   End WithPhoasMap.
+
+  (* Remove one occurrence of x from l if there is one.
+   * Auxiliary function for the definition of fresh' below *)
+  Fixpoint remove_one (x : string) (l : list string) : list string :=
+    match l with
+    | nil => nil
+    | h :: t => if eqb h x then t else h :: remove_one x t
+    end.
+
+  Lemma in_remove_one_len : forall (x : string) (l : list string),
+      In x l -> List.length l = S (List.length (remove_one x l)).
+  Proof.
+    intros. induction l.
+    - apply in_nil in H. exfalso. apply H.
+    - simpl in H. destruct (eqb a x) eqn:E.
+      + simpl. rewrite E. reflexivity.
+      + destruct H as [HL | HR].
+        * rewrite <- eqb_eq in HL. rewrite HL in E. discriminate.
+        * simpl. rewrite E. simpl. rewrite (IHl HR). reflexivity.
+  Qed.
+
+  Lemma in_remove_one : forall (x : string) (l : list string),
+      In x l -> forall (y : string), x = y \/ In x (remove_one y l).
+  Proof.
+    intros x l H. induction l.
+    - intros. apply in_nil in H. exfalso. exact H.
+    - intros y. simpl in H. destruct H as [HL | HR].
+      + destruct (eqb a y) eqn:E.
+        * rewrite eqb_eq in E. rewrite HL in E. left. exact E.
+        * right. simpl. rewrite E. simpl. left. exact HL.
+      + destruct (IHl HR) with (y := y) as [HL' | HR'].
+        * left. exact HL'.
+        * right. simpl. destruct (eqb a y) eqn:E.
+          { exact HR. }
+          { simpl. right. exact HR'. }
+  Qed.
+
+  (* Append "'"s to x until the resulting name is not in used.
+   * The initial call should have (budget = length used) *)
+  Fixpoint fresh' (budget : nat) (used : list string) (x : string) : string :=
+    (* We need budget as a decreasing argument for the function *)
+    match budget with
+    | O => x
+    | S n => match in_dec string_dec x used with
+             | left _ => fresh' n (remove_one x used) (x ++ "'")
+             | right _ => x
+             end
+    end.
+
+  (* Given a list of used names and a hint, return a fresh name *)
+  Definition fresh (used : list string) (x : string) : string :=
+    fresh' (List.length used) used x.
+
+  Lemma len_app : forall y, length y < length (y ++ "'").
+  Proof.
+    induction y; auto. simpl. apply Arith_prebase.lt_n_S_stt. apply IHy.
+  Qed.
+
+  Lemma fresh'_len : forall (budget : nat) (used : list string) (x : string),
+      length x <= length (fresh' budget used x).
+  Proof.
+    induction budget; intros.
+    - destruct used; unfold fresh'; constructor.
+    - destruct (in_dec string_dec x used) eqn:E.
+      + unfold fresh'. rewrite E.
+        apply Nat.le_trans with (m := length (x ++ "'")).
+        * pose proof (len_app x) as len_app_x.
+          apply Nat.lt_le_incl. exact len_app_x.
+        * apply (IHbudget (remove_one x used) (x ++ "'")%string).
+      + unfold fresh'; rewrite E; constructor.
+  Qed.
+
+  Lemma fresh'_is_fresh : forall (budget : nat) (used : list string) (x : string),
+      budget = List.length used -> ~ In (fresh' budget used x) used.
+  Proof.
+    induction budget; intros.
+    - destruct used.
+      + auto.
+      + discriminate.
+    - rewrite H. destruct (in_dec string_dec x used) as [ HL | HR ] eqn:E.
+      + assert (Hrm_len: S budget = S (List.length (remove_one x used))).
+        { rewrite H. apply in_remove_one_len. apply HL. }
+        injection Hrm_len as Hrm_len.
+        apply (IHbudget (remove_one x used)) with (x := (x ++ "'")%string) in Hrm_len as Hrm.
+        unfold not. intros. apply in_remove_one with (y := x) in H0 as [HL'|HR'].
+        * assert (HA : length (x ++ "'") <= length (fresh' (Datatypes.length used) used x)).
+          { unfold fresh'. rewrite <- H. rewrite E. apply fresh'_len. }
+          rewrite HL' in HA. apply Arith_prebase.le_not_lt_stt in HA.
+          apply HA. apply len_app.
+        * unfold fresh' in HR'. rewrite <- H in HR'. rewrite E in HR'.
+          apply Hrm. unfold fresh'. apply HR'.
+      + unfold fresh'. rewrite <- H. rewrite E. exact HR.
+  Qed.
+
+  Corollary fresh_is_fresh : forall (used : list string) (x : string), ~ In (fresh used x) used.
+  Proof.
+    intros. unfold fresh. apply fresh'_is_fresh. reflexivity.
+  Qed.
 
   Definition const_string : type -> Type := fun _ => string.
 
@@ -199,17 +199,6 @@ Section WithMap.
     end.
 
   Context {tenv : map.map string (type * bool)} {tenv_ok : map.ok tenv}.
-  Context {tstore : map.map string type} {tstore_ok : map.ok tenv}.
-
-  Definition phoasify_envs_consistent (G : tenv) (l : locals) (env : locals) (store : locals) : Prop :=
-    forall x,
-      match map.get G x, map.get l x with
-      | Some (t, is_mut), Some v =>
-          let m := if is_mut then store else env in
-          map.get m x = Some v /\ projT1 v = t
-      | Some _, None => False
-      | None, _ => True
-      end.
 
   Lemma eq_dec_refl : forall  {t : Type} (eq_dec : forall (v1 v2 : t), {v1 = v2} + {v1 <> v2}),
     forall (x : t), eq_dec x x = left eq_refl.
@@ -219,60 +208,113 @@ Section WithMap.
     - exfalso. apply n. reflexivity.
   Qed.
 
-  Lemma phoasify_envs_consistent_immut_step : forall G l env store x t (v : interp_type t), phoasify_envs_consistent G l env store -> phoasify_envs_consistent (map.put G x (t, false)) (set_local l x v) (set_phoas_local env x v) store.
-  Proof.
-    unfold phoasify_envs_consistent. intros. unfold set_local. unfold set_phoas_local. destruct (string_dec x0 x).
-    - subst. repeat rewrite map.get_put_same. eauto.
-    - repeat rewrite map.get_put_diff by assumption. pose proof (H x0) as H0.
-      destruct (map.get G x0) eqn:E; auto. destruct p as [t' b]. destruct b.
-      + exact H0.
-      + rewrite map.get_put_diff by assumption. exact H0.
-  Qed.
-
   Ltac eq_projT2_eq := match goal with
                        | H : existT ?f ?t _ = existT ?f ?t _ |- _ =>
                            apply Eqdep_dec.inj_pair2_eq_dec in H;[ subst; eauto | apply type_eq_dec]
                        end.
 
-  Lemma phoasify_sound' :
-    forall {t : type} (e : expr t) (G : tenv),
-      wf G e ->
-      forall (l env store : locals),
-        phoasify_envs_consistent G l env store ->
-        interp_expr l e = interp_phoas_expr store (phoasify env e).
-  Proof.
-    induction e; intros; simpl.
-    - unfold get_local. inversion H. unfold phoasify_envs_consistent in H0.
-      pose proof (H0 x) as Hx. rewrite H4 in Hx. unfold phoas_proj_expected.
-      destruct (map.get l x).
-      + destruct Hx. unfold proj_expected. subst. rewrite H5.
-        rewrite (eq_dec_refl type_eq_dec). reflexivity.
-      + exfalso. exact Hx.
-    - unfold get_local. inversion H. unfold phoasify_envs_consistent in H0.
-      pose proof (H0 x) as Hx. rewrite H4 in Hx. unfold phoas_proj_expected.
-      destruct (map.get l x).
-      + destruct  Hx. unfold proj_expected. subst. rewrite H5.
-        rewrite (eq_dec_refl type_eq_dec). reflexivity.
-      + exfalso. exact Hx.
-    - reflexivity.
-    - f_equal. inversion H. eq_projT2_eq.
-    - inversion H; subst; repeat eq_projT2_eq. f_equal; eauto.
-    - inversion H; repeat eq_projT2_eq. f_equal.
-      + extensionality y. apply (IHe2 _ H8). apply phoasify_envs_consistent_immut_step. assumption.
-      + eapply (IHe1 G); assumption.
-    - inversion H; repeat eq_projT2_eq. f_equal.
-      + extensionality v. extensionality acc. apply (IHe3 _ H11).
-        repeat apply phoasify_envs_consistent_immut_step. assumption.
-      + apply (IHe2 G); assumption.
-      + apply (IHe1 G); assumption.
-    - inversion H; repeat eq_projT2_eq. destruct (interp_expr l e1) eqn:E;
-        rewrite (IHe1 _ H6 _ _ _ H0) in E; rewrite E.
-      + apply (IHe2 _ H7 _ _ _ H0).
-      + apply (IHe3 _ H8 _ _ _ H0).
-    - inversion H; repeat eq_projT2_eq.
-      rewrite (IHe1 _ H5 _ _ _ H0).
-      apply (IHe2 _ H8). apply phoasify_envs_consistent_immut_step. exact H0.
-  Qed.
+  Section WithPhoasEnv.
+    Context {phoas_env : forall V, map.map string {t : type & V t}} {phoas_env_ok : forall V, map.ok (phoas_env V)}.
+
+    Definition phoasify_envs_consistent (G : tenv) (l : locals) (env : phoas_env interp_type) (store : locals) : Prop :=
+      forall x,
+        match map.get G x, map.get l x with
+        | Some (t, is_mut), Some v =>
+            if is_mut then map.get store x = Some v  /\ projT1 v = t
+            else  map.get env x = Some v  /\ projT1 v = t
+        | Some _, None => False
+        | None, _ => True
+        end.
+
+    Lemma phoasify_envs_consistent_immut_step : forall G l env store x t (v : interp_type t), phoasify_envs_consistent G l env store -> phoasify_envs_consistent (map.put G x (t, false)) (set_local l x v) (set_phoas_local env x v) store.
+    Proof.
+      unfold phoasify_envs_consistent. intros. unfold set_local. unfold set_phoas_local. destruct (string_dec x0 x).
+      - subst. repeat rewrite map.get_put_same; eauto.
+      - repeat rewrite map.get_put_diff by assumption. pose proof (H x0) as H0.
+        destruct (map.get G x0) eqn:E; auto.
+    Qed.
+
+    Lemma phoasify_sound' :
+      forall {t : type} (e : expr t) (G : tenv),
+        wf G e ->
+        forall (l : locals) (env : phoas_env interp_type) (store : locals),
+          phoasify_envs_consistent G l env store ->
+          interp_expr l e = interp_phoas_expr store (phoasify env e).
+    Proof.
+      induction e; intros; simpl.
+      - unfold get_local. inversion H. unfold phoasify_envs_consistent in H0.
+        pose proof (H0 x) as Hx. rewrite H4 in Hx. unfold phoas_proj_expected.
+        destruct (map.get l x).
+        + destruct Hx. unfold proj_expected. subst. rewrite H5.
+          rewrite (eq_dec_refl type_eq_dec). reflexivity.
+        + exfalso. exact Hx.
+      - unfold get_local. inversion H. unfold phoasify_envs_consistent in H0.
+        pose proof (H0 x) as Hx. rewrite H4 in Hx. unfold phoas_proj_expected.
+        destruct (map.get l x).
+        + destruct  Hx. unfold proj_expected. subst. rewrite H5.
+          rewrite (eq_dec_refl type_eq_dec). reflexivity.
+        + exfalso. exact Hx.
+      - reflexivity.
+      - f_equal. inversion H. eq_projT2_eq.
+      - inversion H; subst; repeat eq_projT2_eq. f_equal; eauto.
+      - inversion H; repeat eq_projT2_eq. f_equal.
+        + extensionality y. apply (IHe2 _ H8). apply phoasify_envs_consistent_immut_step. assumption.
+        + eapply (IHe1 G); assumption.
+      - inversion H; repeat eq_projT2_eq. f_equal.
+        + extensionality v. extensionality acc. apply (IHe3 _ H11).
+          repeat apply phoasify_envs_consistent_immut_step. assumption.
+        + apply (IHe2 G); assumption.
+        + apply (IHe1 G); assumption.
+      - inversion H; repeat eq_projT2_eq. destruct (interp_expr l e1) eqn:E;
+          rewrite (IHe1 _ H6 _ _ _ H0) in E; rewrite E.
+        + apply (IHe2 _ H7 _ _ _ H0).
+        + apply (IHe3 _ H8 _ _ _ H0).
+      - inversion H; repeat eq_projT2_eq.
+        rewrite (IHe1 _ H5 _ _ _ H0).
+        apply (IHe2 _ H8). apply phoasify_envs_consistent_immut_step. exact H0.
+    Qed.
+
+    Definition Phoasify {t : type} (e : expr t) : Phoas_expr t:=
+      fun (V : type -> Type) => phoasify (V := V) map.empty e.
+
+    Definition phoasify_envs_consistent_closed (G : tenv) (l store : locals) : Prop :=
+      forall x, match map.get G x with
+                | Some (t, true) =>
+                    match map.get l x with
+                    | Some v => map.get store x = Some v /\ projT1 v = t
+                    | None => False
+                    end
+                | _ => True
+                end.
+
+    Definition Flat_wf (G : tenv) {t : type} (e : expr t) :=
+      (forall x, match map.get G x with
+                 | Some (t, is_mut) =>
+                     (* All variables are mutable *)
+                     is_mut = true
+                 | None => True
+                 end) /\
+        wf G e.
+
+    Theorem phoasify_sound : forall {t : type} (e : expr t) (G : tenv),
+        Flat_wf G e ->
+        forall l store : locals,
+          phoasify_envs_consistent_closed G l store ->
+          interp_expr l e = interp_phoas_expr store (Phoasify e interp_type).
+    Proof.
+      intros t e G [H_closed H_wf] l store H_consistent_closed.
+      assert (H_consistent : phoasify_envs_consistent G l map.empty store).
+      { unfold phoasify_envs_consistent. intro x.
+        pose proof (H_closed x) as H_closed'.
+        pose proof (H_consistent_closed x) as H_consistent_closed'.
+        destruct (map.get G x) eqn:E; trivial. destruct p. subst.
+        assumption.
+      }
+      unfold Phoasify. eapply phoasify_sound'.
+      - apply H_wf.
+      - assumption.
+    Qed.
+  End WithPhoasEnv.
 
   Section expr_equiv.
     Context {V V' : type -> Type}.
@@ -320,201 +362,182 @@ Section WithMap.
     (* Typing environment for mutable variables *)
     Context {tenv_mut : map.map string type} {tenv_mut_ok : map.ok tenv_mut}.
 
-  Inductive phoas_wf {V : type -> Type} : tenv_mut -> forall {t : type}, phoas_expr V t -> Prop :=
-  | wf_PhEVar G t v : phoas_wf G (PhEVar t v)
-  | wf_PhELoc G t x :
-    map.get G x = Some t ->
-    phoas_wf G (PhELoc t x)
-  | wf_PhEAtom G {t} (a : atom t) : phoas_wf G (PhEAtom a)
-  | wf_PhEUnop G {t1 t2} (o : unop t1 t2) e :
-    phoas_wf G e ->
-    phoas_wf G (PhEUnop o e)
-  | wf_PhEBinop G {t1 t2 t3} (o : binop t1 t2 t3) e1 e2 :
-    phoas_wf G e1 ->
-    phoas_wf G e2 ->
-    phoas_wf G (PhEBinop o e1 e2)
-  | wf_PhEFlatmap G {t1 t2} l1 x (fn_l2 : V t1 -> phoas_expr V (TList t2)) :
-    phoas_wf G l1 ->
-    (forall v, phoas_wf G (fn_l2 v)) ->
-    phoas_wf G (PhEFlatmap l1 x fn_l2)
-  | wf_PhEFold G {t1 t2} l1 e2 x y (fn_e3 : V t1 -> V t2 -> phoas_expr V t2) :
-    phoas_wf G l1 ->
-    phoas_wf G e2 ->
-    (forall v1 v2, phoas_wf G (fn_e3 v1 v2)) ->
-    phoas_wf G (PhEFold l1 e2 x y fn_e3)
-  | wf_PhEIf G {t} e1 (e2 e3 : phoas_expr V t) :
-    phoas_wf G e1 ->
-    phoas_wf G e2 ->
-    phoas_wf G e3 ->
-    phoas_wf G (PhEIf e1 e2 e3)
-  | wf_PhELet G {t1 t2} x e1 (fn_e2 : V t1 -> phoas_expr V t2) :
-    phoas_wf G e1 ->
-    (forall v, phoas_wf G (fn_e2 v)) ->
-    phoas_wf G (PhELet x e1 fn_e2).
+    Inductive phoas_wf {V : type -> Type} : tenv_mut -> forall {t : type}, phoas_expr V t -> Prop :=
+    | wf_PhEVar G t v : phoas_wf G (PhEVar t v)
+    | wf_PhELoc G t x :
+      map.get G x = Some t ->
+      phoas_wf G (PhELoc t x)
+    | wf_PhEAtom G {t} (a : atom t) : phoas_wf G (PhEAtom a)
+    | wf_PhEUnop G {t1 t2} (o : unop t1 t2) e :
+      phoas_wf G e ->
+      phoas_wf G (PhEUnop o e)
+    | wf_PhEBinop G {t1 t2 t3} (o : binop t1 t2 t3) e1 e2 :
+      phoas_wf G e1 ->
+      phoas_wf G e2 ->
+      phoas_wf G (PhEBinop o e1 e2)
+    | wf_PhEFlatmap G {t1 t2} l1 x (fn_l2 : V t1 -> phoas_expr V (TList t2)) :
+      phoas_wf G l1 ->
+      (forall v, phoas_wf G (fn_l2 v)) ->
+      phoas_wf G (PhEFlatmap l1 x fn_l2)
+    | wf_PhEFold G {t1 t2} l1 e2 x y (fn_e3 : V t1 -> V t2 -> phoas_expr V t2) :
+      phoas_wf G l1 ->
+      phoas_wf G e2 ->
+      (forall v1 v2, phoas_wf G (fn_e3 v1 v2)) ->
+      phoas_wf G (PhEFold l1 e2 x y fn_e3)
+    | wf_PhEIf G {t} e1 (e2 e3 : phoas_expr V t) :
+      phoas_wf G e1 ->
+      phoas_wf G e2 ->
+      phoas_wf G e3 ->
+      phoas_wf G (PhEIf e1 e2 e3)
+    | wf_PhELet G {t1 t2} x e1 (fn_e2 : V t1 -> phoas_expr V t2) :
+      phoas_wf G e1 ->
+      (forall v, phoas_wf G (fn_e2 v)) ->
+      phoas_wf G (PhELet x e1 fn_e2).
 
-  Definition projT1_snd_T2 {A : Type} {P1 P2 : A -> Type} (v : {t : A & (P1 t * P2 t)%type}) :
-    {t : A & P2 t} :=
-    existT _ (projT1 v) (snd (projT2 v)).
+    Definition projT1_snd_T2 {A : Type} {P1 P2 : A -> Type} (v : {t : A & (P1 t * P2 t)%type}) :
+      {t : A & P2 t} :=
+      existT _ (projT1 v) (snd (projT2 v)).
 
-  Definition dephoasify_envs_consistent (C : ctxt) (G : tenv_mut) (store l : locals) (used : list string) :=
-    (forall (p : {t : type & (string * interp_type t)%type}),
-        In p C ->
-        let s := fst (projT2 p) in
-        In s used /\
-          (* Immutable variable name not used as mutable variable *)
-          match map.get G s with
-          | Some _ => False
-          | None => True
-          end /\
-          match map.get l s with
-          | Some p' => projT1_snd_T2 p = p'
-          | None => False
-          end)
-    /\ (forall s, match map.get G s with
-                  | Some t => In s used /\
-                                match map.get store s with
-                                | Some p => projT1 p = t /\ map.get l s = Some p
-                                | None => False
-                                end
-                  | None => True
-                  end).
+    Definition dephoasify_envs_consistent (C : ctxt) (G : tenv_mut) (store l : locals) (used : list string) :=
+      (forall (p : {t : type & (string * interp_type t)%type}),
+          In p C ->
+          let s := fst (projT2 p) in
+          In s used /\
+            (* Immutable variable name not used as mutable variable *)
+            match map.get G s with
+            | Some _ => False
+            | None => True
+            end /\
+            match map.get l s with
+            | Some p' => projT1_snd_T2 p = p'
+            | None => False
+            end)
+      /\ (forall s, match map.get G s with
+                    | Some t => In s used /\
+                                  match map.get store s with
+                                  | Some p => projT1 p = t /\ map.get l s = Some p
+                                  | None => False
+                                  end
+                    | None => True
+                    end).
 
-  Lemma dephoasify_envs_consistent_immut_step: forall C G store l used t x y,
-      dephoasify_envs_consistent C G store l used ->
-      ~ In x used ->
-      dephoasify_envs_consistent (vars t (x, y) :: C) G store (set_local l x y) (x :: used).
-  Proof.
-    intros C G store l used t x y [HL HR] H_not_in. split.
-    - intros p [H_inL | H_inR].
-      + subst; simpl. unfold set_local. rewrite map.get_put_same.
-        unfold projT1_snd_T2. simpl. split;
-          [left | split]; try reflexivity.
-        pose proof (HR x) as HRx. destruct (map.get G x); trivial.
-        destruct HRx as [HRL _]. apply H_not_in. assumption.
-      + apply HL in H_inR. remember (fst (projT2 p)) as s; simpl.
-        unfold set_local. destruct H_inR. split; [right; assumption |].
-        rewrite map.get_put_diff; [assumption | congruence].
-    - intro s. pose proof (HR s) as HRs. destruct (map.get store s) eqn:E.
-      + unfold set_local. destruct (map.get G s); trivial. destruct HRs; split.
-        * right; assumption.
-        * rewrite map.get_put_diff; [assumption | congruence].
-      + destruct (map.get G s); [destruct HRs; exfalso; assumption | trivial].
-  Qed.
-
-  Lemma dephoasify_envs_consistent_used_step: forall C G store l used x,
-      dephoasify_envs_consistent C G store l used ->
-      dephoasify_envs_consistent C G store l (x::used).
-  Proof.
-    intros C G store l used x [HL HR]. simpl in *.
-    unfold dephoasify_envs_consistent. split.
-    - intros p H. pose proof (HL p H) as [HL1 [HL2 HL3]].
-      split; [right | split]; assumption.
-    - intro s. pose proof (HR s) as HR'.
-      destruct (map.get G s); destruct HR'; trivial.
-      split; [right | ]; assumption.
-  Qed.
-
-  Lemma dephoasify_sound' :
-    forall {t : type} (e : phoas_expr const_string t) (e0 : phoas_expr interp_type t) (C : ctxt),
-      phoas_expr_equiv C e e0 ->
-      forall (G : tenv_mut),
-        phoas_wf G e ->
-        forall (store l : locals) (used : list string),
+    Lemma dephoasify_envs_consistent_immut_step: forall C G store l used t x y,
         dephoasify_envs_consistent C G store l used ->
-        interp_phoas_expr store e0 = interp_expr l (dephoasify used e).
-  Proof.
-    induction e; intros e0 C H_equiv G H_wf store l used H_consistent; simpl;
-      inversion H_equiv; subst; repeat eq_projT2_eq; simpl.
-    - unfold get_local. apply H_consistent in H3 as [_ [_ H3]]. simpl in H3.
-      destruct (map.get l v).
-      + unfold proj_expected. subst. simpl. rewrite (eq_dec_refl type_eq_dec). reflexivity.
-      + exfalso; assumption.
-    - inversion H_wf. subst. destruct H_consistent as [_ HR]. unfold get_local.
-      pose proof (HR x') as HR'. rewrite H2 in HR'; destruct HR' as [_ HR'].
-      destruct (map.get store x') eqn:E.
-      + destruct (map.get l x'); destruct HR' as [HR'L HR'R];
-          [injection HR'R as HR'R; congruence | discriminate].
-      + exfalso; assumption.
-    - inversion H_equiv; inversion H_wf. repeat eq_projT2_eq. f_equal. eauto.
-    - inversion H_equiv; inversion H_wf. repeat eq_projT2_eq. simpl. f_equal; eauto.
-    - inversion H_equiv; inversion H_wf. repeat eq_projT2_eq. f_equal.
-      + extensionality y. eapply H.
-        * apply H8.
-        * apply H20.
-        * apply dephoasify_envs_consistent_immut_step;
-            [assumption | apply fresh_is_fresh].
-      + eapply IHe.
-        * apply H4.
-        * apply H17.
-        * apply dephoasify_envs_consistent_used_step. assumption.
-    - inversion H_equiv; inversion H_wf. repeat eq_projT2_eq. f_equal.
-      + extensionality v. extensionality acc.
+        ~ In x used ->
+        dephoasify_envs_consistent (vars t (x, y) :: C) G store (set_local l x y) (x :: used).
+    Proof.
+      intros C G store l used t x y [HL HR] H_not_in. split.
+      - intros p [H_inL | H_inR].
+        + subst; simpl. unfold set_local. rewrite map.get_put_same.
+          unfold projT1_snd_T2. simpl. split;
+            [left | split]; try reflexivity.
+          pose proof (HR x) as HRx. destruct (map.get G x); trivial.
+          destruct HRx as [HRL _]. apply H_not_in. assumption.
+        + apply HL in H_inR. remember (fst (projT2 p)) as s; simpl.
+          unfold set_local. destruct H_inR. split; [right; assumption |].
+          rewrite map.get_put_diff; [assumption | congruence].
+      - intro s. pose proof (HR s) as HRs. destruct (map.get store s) eqn:E.
+        + unfold set_local. destruct (map.get G s); trivial. destruct HRs; split.
+          * right; assumption.
+          * rewrite map.get_put_diff; [assumption | congruence].
+        + destruct (map.get G s); [destruct HRs; exfalso; assumption | trivial].
+    Qed.
+
+    Lemma dephoasify_envs_consistent_used_step: forall C G store l used x,
+        dephoasify_envs_consistent C G store l used ->
+        dephoasify_envs_consistent C G store l (x::used).
+    Proof.
+      intros C G store l used x [HL HR]. simpl in *.
+      unfold dephoasify_envs_consistent. split.
+      - intros p H. pose proof (HL p H) as [HL1 [HL2 HL3]].
+        split; [right | split]; assumption.
+      - intro s. pose proof (HR s) as HR'.
+        destruct (map.get G s); destruct HR'; trivial.
+        split; [right | ]; assumption.
+    Qed.
+
+    Lemma dephoasify_sound' :
+      forall {t : type} (e : phoas_expr const_string t) (e0 : phoas_expr interp_type t) (C : ctxt),
+        phoas_expr_equiv C e e0 ->
+        forall (G : tenv_mut),
+          phoas_wf G e ->
+          forall (store l : locals) (used : list string),
+            dephoasify_envs_consistent C G store l used ->
+            interp_phoas_expr store e0 = interp_expr l (dephoasify used e).
+    Proof.
+      induction e; intros e0 C H_equiv G H_wf store l used H_consistent; simpl;
+        inversion H_equiv; inversion H_wf; subst; repeat eq_projT2_eq; simpl.
+      - unfold get_local. apply H_consistent in H3 as [_ [_ H3]]. simpl in H3.
+        destruct (map.get l v).
+        + unfold proj_expected. subst. simpl. rewrite (eq_dec_refl type_eq_dec). reflexivity.
+        + exfalso; assumption.
+      - inversion H_wf. subst. destruct H_consistent as [_ HR]. unfold get_local.
+        pose proof (HR x') as HR'. rewrite H2 in HR'; destruct HR' as [_ HR'].
+        destruct (map.get store x') eqn:E.
+        + destruct (map.get l x'); destruct HR' as [HR'L HR'R];
+            [injection HR'R as HR'R; congruence | discriminate].
+        + exfalso; assumption.
+      - f_equal; eauto.
+      - f_equal; eauto.
+      - f_equal.
+        + extensionality y. eapply H.
+          * apply H8.
+          * apply H16.
+          * apply dephoasify_envs_consistent_immut_step;
+              [assumption | apply fresh_is_fresh].
+        + eapply IHe.
+          * apply H4.
+          * apply H13.
+          * apply dephoasify_envs_consistent_used_step. assumption.
+      - f_equal; eauto.
+        extensionality v. extensionality acc.
         eapply H; try eauto.
         repeat apply dephoasify_envs_consistent_immut_step;
           try apply fresh_is_fresh. assumption.
-      + eauto.
-      + eauto.
-    - inversion H_equiv; inversion H_wf. repeat eq_projT2_eq.
-      erewrite IHe1 by eauto. erewrite IHe2 by eauto. erewrite IHe3 by eauto.
-      reflexivity.
-    - inversion H_equiv; inversion H_wf. repeat eq_projT2_eq.
-      eapply H; eauto. erewrite IHe by eauto.
-      apply dephoasify_envs_consistent_immut_step;
-        [assumption | apply fresh_is_fresh].
-  Qed.
+      - erewrite IHe1 by eauto. erewrite IHe2 by eauto. erewrite IHe3 by eauto.
+        reflexivity.
+      - eapply H; eauto. erewrite IHe by eauto.
+        apply dephoasify_envs_consistent_immut_step;
+          [assumption | apply fresh_is_fresh].
+    Qed.
 
-  Definition Flat_wf (G : tenv) {t : type} (e : expr t) :=
-    (forall x, match map.get G x with
-               | Some (t, is_mut) =>
-                   (* All variables are mutable *)
-                   is_mut = true
-               | None => True
-               end) /\
-      wf G e.
+    Definition Dephoasify (used : list string) {t : type} (e : Phoas_expr t) : expr t :=
+      dephoasify used (e const_string).
 
-  Definition phoasify_envs_consistent_closed (G : tenv) (l store : locals) : Prop :=
-    forall x, match map.get G x with
-              | Some (t, true) =>
-                    match map.get l x with
-                    | Some v => map.get store x = Some v /\ projT1 v = t
-                    | None => False
-                    end
-              | _ => True
-              end.
+    Definition dephoasify_envs_consistent_closed (G : tenv_mut) (store l : locals) (used : list string) : Prop :=
+      forall s : string, match map.get G s with
+                         | Some t => In s used /\
+                                       match map.get store s with
+                                       | Some p => projT1 p = t /\ map.get l s = Some p
+                                       | None => False
+                                       end
+                         | None => True
+                         end.
 
-  Theorem phoasify_sound : forall {t : type} (e : expr t) (G : tenv),
-      Flat_wf G e ->
-      forall l store : locals,
-        phoasify_envs_consistent_closed G l store ->
-        interp_expr l e = interp_phoas_expr store (phoasify map.empty e).
-  Abort.
+    Definition Phoas_wf (G : tenv_mut) {t : type} (e : Phoas_expr t) :=
+      (forall V1 V2, phoas_expr_equiv nil (e V1) (e V2)) /\
+        forall V, phoas_wf G (e V).
 
-  Definition dephoasify_envs_consistent_closed (G : tenv_mut) (store l : locals) (used : list string) : Prop :=
-    forall s : string, match map.get G s with
-                       | Some t => In s used /\
-                                     match map.get store s with
-                                     | Some p => projT1 p = t /\ match map.get l s with
-                                                                | Some p' => p = p'
-                                                                | None => False
-                                                                end
-                                     | None => False
-                                     end
-                       | None => True
-                       end.
+    Theorem dephoasify_sound : forall {t : type} (e : Phoas_expr t) (G : tenv_mut) ,
+        Phoas_wf G e ->
+        forall (store l : locals) (used : list string),
+          dephoasify_envs_consistent_closed G store l used ->
+          interp_phoas_expr store (e interp_type) = interp_expr l (Dephoasify used e).
+    Proof.
+      intros t e G [H_equiv H_wf] store l used H_consistent_closed.
+      eapply dephoasify_sound'.
+      - apply H_equiv.
+      - apply H_wf.
+      - unfold dephoasify_envs_consistent. split.
+        + intros p contra. apply in_nil in contra. exfalso; assumption.
+        + assumption.
+    Qed.
 
-  Definition Phoas_wf (G : tenv_mut) {t : type} (e : Phoas_expr t) :=
-    (forall V1 V2, phoas_expr_equiv nil (e V1) (e V2)) /\
-  forall V, phoas_wf G (e V).
+  End WithPhoasTypeEnv.
+End WithMap.
 
-  Theorem dephoasify_sound : forall {t : type} (e : Phoas_expr t) (G : tenv_mut) ,
-      Phoas_wf G e ->
-      forall (store l : locals) (used : list string),
-        dephoasify_envs_consistent_closed G store l used ->
-        interp_phoas_expr store (e interp_type) = interp_expr l (dephoasify used (e const_string)).
-Abort.
-    (* =============== Wip =============== *)
-  (* TODO: move eq_dec_refl elsewhere
+
+(* TODO: move eq_dec_refl elsewhere
 Flat_wf to Phoas_wf and vice versa
+Try out separated tenv into mut and immut? By an auxiliary file instead of refactoring?
 mem for bare metal; store for mutable; env for immutable *)
-End WithPhoasTypeEnv.
-  End WithMap.
